DS/TernarySearchTree.v
@@ -1,0 +1,6 @@
+(** Ternary Search Tree (a data structure for storing finite collections
+    of strings:
+
+    https://www.drdobbs.com/database/ternary-search-trees/184410528
+
+*)
